24/12/06 Lean 4 4.15.0-rc1 に更新

Divseq2/Lean/Basic.lean
@@ -1,4 +1,3 @@
-import Mathlib.Tactic.LibrarySearch
 import Mathlib.Tactic.Linarith
 
 #eval Lean.versionString
@@ -26,7 +25,7 @@ def mod3 (n : Nat) : Mod3 n := match n with
     | Mod3.threeOne k  => Mod3.threeTwo k
     | Mod3.threeTwo k  => by rw[←m₁]; exact Mod3.threeZero (succ k)
 
-def allDivSeq (x:Nat) : List (List Integer) := [[]] -- TBD
+def allDivSeq (x:Nat) : List (List Int) := [[]] -- TBD
 
 inductive ExtsLimited : Nat → Prop where
   | is : (l : Nat)
@@ -36,32 +35,29 @@ inductive ExtsLimited : Nat → Prop where
       → (ExtsLimited <| succ (succ (succ (l * 2 * 3))))                     -- 11
       → (ExtsLimited <| 18*l+13)                                            -- 03'
       → (ExtsLimited <| 9*l+6)                                              -- 12'
-      → (ExtsLimited <| l+(l-3)/8+1)                                        -- 06' 割り算も計算すると Nat に落ち着くので問題無し
+      → (ExtsLimited <| l+(l-3)/8+1)                                        -- 06'
       → (ExtsLimited <| l+(l-4)/4*5+6)                                      -- 07'
       → (ExtsLimited <| 4*l+(l-3)/2+4)                                      -- 08'
       → (ExtsLimited <| 9*l+16)                                             -- 04'
-      → (ExtsLimited <| (9*l+11)/2)                                          -- 05'
+      → (ExtsLimited <| (9*l+11)/2)                                         -- 05'
       → (ExtsLimited <| (9*l+15)/2)                                         -- 13'
       → (ExtsLimited <| (9*l+9)/4)                                          -- 14'
         → (ExtsLimited <| l)
 
 inductive SingleLimited : Nat → Prop where
-  | is02 : (l : Nat) → (ExtsLimited <| l) → (SingleLimited <| succ (succ (succ (succ ((succ (l * 2 * 2)) * 3)))))
-  | is03 : (m : Nat) → (ExtsLimited <| 2*m) → (SingleLimited <| succ (succ (succ (succ ((succ ((succ (m * 3 * 2)) * 2)) * 3)))))
-  | is04 : (m : Nat) → (ExtsLimited <| 4*m+1) → (SingleLimited <| succ (succ (succ (succ (succ (succ (succ (m * 3) * 2) * 2) * 3)))))
-  | is05 : (m : Nat) → (ExtsLimited <| 8*m+7) → (SingleLimited <| succ (succ (succ (succ (succ (succ (succ (succ (m * 3)) * 2) * 2) * 3)))))
+  | is02 : (l : Nat) → (ExtsLimited <| l)      → (SingleLimited <| succ (succ (succ (succ ((succ (l * 2 * 2)) * 3)))))
+  | is03 : (m : Nat) → (ExtsLimited <| 2*m)    → (SingleLimited <| succ (succ (succ (succ ((succ ((succ (m * 3 * 2)) * 2)) * 3)))))
+  | is04 : (m : Nat) → (ExtsLimited <| 4*m+1)  → (SingleLimited <| succ (succ (succ (succ (succ (succ (succ (m * 3) * 2) * 2) * 3)))))
+  | is05 : (m : Nat) → (ExtsLimited <| 8*m+7)  → (SingleLimited <| succ (succ (succ (succ (succ (succ (succ (succ (m * 3)) * 2) * 2) * 3)))))
   | is06 : (l : Nat) → (ExtsLimited <| 16*l+3) → (SingleLimited <| succ (succ (succ (succ (l * 3 * 2 * 3)))))
-  | is07 : (l : Nat) → (ExtsLimited <| 8*l+4) → (SingleLimited <| succ (succ (succ (succ (((succ (l * 3)) * 2) * 3)))))
-  | is08 : (l : Nat) → (ExtsLimited <| 4*l+3) → (SingleLimited <| succ (succ (succ (succ (((succ (succ (l * 3))) * 2) * 3)))))
-  | is09 : (j : Nat) → (ExtsLimited <| j) → (SingleLimited <| succ (succ (j*3)))
-  | is11 : (k : Nat) → (ExtsLimited <| k) → (SingleLimited <| succ (succ (succ (k * 2 * 3))))
-  | is12 : (l : Nat) → (ExtsLimited <| 2*l) → (SingleLimited <| succ (succ (succ ((succ (l * 3 * 2)) * 3))))
-  | is13 : (l : Nat) → (ExtsLimited <| 4*l+1) → (SingleLimited <| succ (succ (succ (succ (succ (l * 3) * 2) * 3))))
-  | is14 : (l : Nat) → (ExtsLimited <| 8*l+7) → (SingleLimited <| succ (succ (succ (succ (succ (succ (l * 3)) * 2) * 3))))
+  | is07 : (l : Nat) → (ExtsLimited <| 8*l+4)  → (SingleLimited <| succ (succ (succ (succ (((succ (l * 3)) * 2) * 3)))))
+  | is08 : (l : Nat) → (ExtsLimited <| 4*l+3)  → (SingleLimited <| succ (succ (succ (succ (((succ (succ (l * 3))) * 2) * 3)))))
+  | is09 : (j : Nat) → (ExtsLimited <| j)      → (SingleLimited <| succ (succ (j*3)))
+  | is11 : (k : Nat) → (ExtsLimited <| k)      → (SingleLimited <| succ (succ (succ (k * 2 * 3))))
+  | is12 : (l : Nat) → (ExtsLimited <| 2*l)    → (SingleLimited <| succ (succ (succ ((succ (l * 3 * 2)) * 3))))
+  | is13 : (l : Nat) → (ExtsLimited <| 4*l+1)  → (SingleLimited <| succ (succ (succ (succ (succ (l * 3) * 2) * 3))))
+  | is14 : (l : Nat) → (ExtsLimited <| 8*l+7)  → (SingleLimited <| succ (succ (succ (succ (succ (succ (l * 3)) * 2) * 3))))
   | is01_2 : ExtsLimited 1 → SingleLimited 1
   | is10_2 : ExtsLimited 0 → SingleLimited 0
 axiom is01 : SingleLimited 1
 axiom is10 : SingleLimited 0
-
-
-
